Cleanup of some rules for crash borrows to ease explanation

src/goose_lang/crash_borrow.v
@@ -120,12 +120,17 @@ Proof.
     iApply (ownfCP_disj with "[$]").
 Qed.
 
-Definition crash_borrow Ps Pc : iProp Σ :=
-  (□ (Ps -∗ Pc) ∗ staged_value_idle ⊤ Ps True%I Pc ∗ later_tok ∗ later_tok).
+Definition pre_borrow : iProp Σ :=
+  (later_tok ∗ later_tok ∗ later_tok ∗ later_tok).
 
-(* This is an "advanced" interface that exposes later tokens *)
-Lemma wpc_crash_borrow_init_toks s k e Φ Φc P Pc :
-  (later_tok ∗ later_tok ∗ later_tok ∗ later_tok) -∗
+Definition crash_borrow Ps Pc : iProp Σ :=
+ (∃ Ps' Pc', □ (Ps -∗ Pc) ∗
+             □ (Ps' -∗ Ps) ∗
+             □ (Pc -∗ Pc') ∗
+             staged_value_idle ⊤ Ps' True%I Pc' ∗ later_tok ∗ later_tok).
+
+Lemma wpc_crash_borrow_inits s k e Φ Φc P Pc :
+  pre_borrow -∗
   P -∗
   □ (P -∗ Pc) -∗
   (crash_borrow P Pc -∗ WPC e @ s; k; ⊤ {{ Φ }} {{ Pc -∗ Φc }}) -∗
@@ -136,15 +141,15 @@ Proof.
   iDestruct "H" as "(Hlt2&Hlt3)".
   iPoseProof (wpc_staged_inv_init _ _ _ _ _ _ P Pc) as "H".
   iSpecialize ("H" with "[$Hlt1 $Hlt2 $HP $Hwand Hwpc Hlt3]").
-  { iIntros. iApply "Hwpc". iFrame. eauto. }
+  { iIntros. iApply "Hwpc". iExists P, Pc. iFrame "# ∗". iSplit; eauto. }
   iApply (wpc_mono with "H"); eauto.
   iIntros "(H1&H2)". by iApply "H1".
 Qed.
 
-Lemma wpc_crash_borrow_generate_tokens s k e Φ Φc :
+Lemma wpc_crash_borrow_generate_pre s k e Φ Φc :
   language.to_val e = None →
   WPC e @ s; k; (⊤ ∖ (↑borrowN : coPset))
-                  {{ v, Nat.iter 4 (λ P : iProp Σ, later_tok ∗ P) True -∗ Φ v }} {{ Φc }} -∗
+                  {{ v, pre_borrow -∗ Φ v }} {{ Φc }} -∗
   WPC e @ s; k; ⊤ {{ Φ }} {{ Φc }}.
 Proof.
   iIntros (Hnv) "Hwpc".
@@ -192,6 +197,18 @@ Proof.
   iSplit; last eauto.
   iIntros (?) "H". iModIntro.
   iApply "H". iFrame.
+Qed.
+
+Lemma wp_crash_borrow_generate_pre s e Φ :
+  language.to_val e = None →
+  WP e @ s; (⊤ ∖ (↑borrowN : coPset))
+                  {{ v, pre_borrow -∗ Φ v }} -∗
+  WP e @ s; ⊤ {{ Φ }}.
+Proof.
+  iIntros (?) "H".
+  iApply (wpc_wp _ 0 _ _ _ True%I).
+  iApply wpc_crash_borrow_generate_pre; auto.
+  iApply (wp_wpc). iApply "H".
 Qed.
 
 Lemma wpc_crash_borrow_init_ctx' s k e Φ Φc P Pc K `{!LanguageCtx K} :
@@ -251,7 +268,9 @@ Proof.
 
   iAssert (crash_borrow P Pc)%I with "[Hlt1 Hlt2 Hlt5 H2 Hstat2 Hitok_u]"  as "Hborrow".
   {
-    iFrame "# ∗".
+    iFrame "# ∗". iExists P, Pc.
+    iSplit; first eauto.
+    iSplit; first eauto.
     iExists _, _, _, _, _, _. iFrame "∗". iFrame "Hsaved Hsaved'".
     iExists _, _. iFrame "Hpri_inv". eauto.
   }
@@ -318,6 +337,21 @@ Proof.
   iIntros "(H1&HP)". iApply "H1". eauto.
 Qed.
 
+Lemma crash_borrow_conseq P Pc P' Pc' :
+  □ (P' -∗ Pc') -∗
+  □ (P -∗ P') -∗
+  □ (Pc' -∗ Pc) -∗
+  crash_borrow P Pc -∗ crash_borrow P' Pc'.
+Proof.
+  iIntros "#Hw1' #Hw2' #Hw3'".
+  iIntros "Hborrow".
+  iDestruct "Hborrow" as (P0 Pc0) "(#Hw1&#Hw2&#H3&Hinv&Htok&Htok')".
+  rewrite /crash_borrow.
+  iExists P0, Pc0. iSplit; first eauto. iFrame "Hinv Htok Htok'".
+  iSplit.
+  - iModIntro. iIntros. iApply "Hw2'". iApply "Hw2". done.
+  - iModIntro. iIntros. iApply "H3". iApply "Hw3'". done.
+Qed.
 
 Lemma wpc_crash_borrow_split k E e Φ Φc P Pc P1 P2 Pc1 Pc2 :
   language.to_val e = None →
@@ -330,7 +364,7 @@ Lemma wpc_crash_borrow_split k E e Φ Φc P Pc P1 P2 Pc1 Pc2 :
   WPC e @ NotStuck; k; E {{ Φ }} {{ Φc }}.
 Proof.
   iIntros (Hnval) "Hborrow Hshift #Hwand1 #Hwand2 Hwandc Hwpc".
-  iDestruct "Hborrow" as "(#Hwand&Hinv&>Htok&>Htok')".
+  iDestruct "Hborrow" as (??) "(#Hw1&#Hw2&#Hw3&Hinv&>Htok&>Htok')".
   iApply (wpc_later_tok_use with "[$]"); first done.
   iNext.
   iApply (wpc_staged_inv_inuse); first done.
@@ -340,7 +374,8 @@ Proof.
     iApply (wpc_crash_modality_wand with "Hwpc").
     iIntros "$". eauto. }
   iIntros "HP".
-  iDestruct ("Hshift" with "[$]") as "(HP1&HP2)".
+  iDestruct ("Hshift" with "[HP]") as "(HP1&HP2)".
+  { iApply "Hw2". eauto. }
   iIntros (mj Hlt).
   iApply wpc_fupd2.
   iApply (wpc_pri_inv_tok_res).
@@ -351,7 +386,7 @@ Proof.
   rewrite wpc_eq. iIntros (mj').
   iApply (wpc0_strong_mono with "Hwpc"); auto.
   iSplit; last first.
-  { iIntros "$ !>". iSplitR; first eauto. iApply "Hwandc". iSplitL "HP1".
+  { iIntros "$ !>". iSplitR; first eauto. iApply "Hw3". iApply "Hwandc". iSplitL "HP1".
     - iApply "Hwand1". eauto.
     - iApply "Hwand2". eauto.
   }
@@ -374,7 +409,10 @@ Proof.
   iDestruct ("Htok") as "(Htok3&Htok)".
   iDestruct ("Htok") as "(Htok4&Htok)".
   iSpecialize ("Hc" with "[Htok1 Htok2 Htok3 Htok4 Hval1 Hval2]").
-  { iFrame "# ∗". }
+  { iSplitL "Htok1 Htok2 Hval1". 
+    - iExists P1, Pc1. iFrame "Hval1". iFrame "#". iFrame. iSplit; eauto.
+    - iExists P2, Pc2. iFrame "Hval2". iFrame "#". iFrame. iSplit; eauto.
+  }
   iDestruct (staged_inv_cancel_wpc_crash_modality with "Hcancel1") as "Hcancel1".
   iDestruct (staged_inv_cancel_wpc_crash_modality with "Hcancel2") as "Hcancel2".
 
@@ -383,7 +421,7 @@ Proof.
   iModIntro. iSplitR "Hc".
   {
     iApply (wpc_crash_modality_wand with "Hcombined").
-    iIntros "(?&?) !>". iApply "Hwandc"; by iFrame.
+    iIntros "(?&?) !>". iApply "Hw3". iApply "Hwandc". by iFrame.
   }
   iSplit.
   - iDestruct "Hc" as "(Hc&_)".
@@ -403,7 +441,7 @@ Lemma wpc_crash_borrow_combine k E e Φ Φc P Pc P1 P2 Pc1 Pc2 :
 Proof.
   iIntros (Hnval) "Hborrow1 Hborrow2 #Hc Hwandc12 HwandP Hwpc".
 
-  iDestruct "Hborrow1" as "(#Hwand1&Hinv1&Htok1&>Htok2)".
+  iDestruct "Hborrow1" as (??) "(#Hw1&#Hw2&#Hw3&Hinv1&Htok1&>Htok2)".
   iApply (wpc_later_tok_use with "[$]"); first done.
   iNext.
   iApply (wpc_staged_inv_inuse2); first done.
@@ -414,7 +452,7 @@ Proof.
     iIntros "$". eauto. }
   iIntros "HP1". iIntros (mj_wp1 Hlt1).
 
-  iDestruct "Hborrow2" as "(#Hwand2&Hinv2&Htok2&_)".
+  iDestruct "Hborrow2" as (??) "(#Hw1'&#Hw2'&#Hw3'&Hinv2&Htok2&_)".
   iApply (wpc_staged_inv_inuse); first done.
   iFrame "Hinv2".
   iSplit.
@@ -422,7 +460,7 @@ Proof.
     iApply (wpc_crash_modality_wand with "Hwpc").
     iIntros "HΦc".
     iModIntro. iFrame. iSplitR; first eauto.
-    iApply wpc_crash_modality_intro. iApply "Hwand1". iFrame. }
+    iApply wpc_crash_modality_intro. iApply "Hw3". iApply "Hw1". iApply "Hw2". iFrame. }
 
   iIntros "HP2". iIntros (mj_wp2 Hlt2).
   iApply wpc_fupd2.
@@ -436,14 +474,17 @@ Proof.
   iApply (wpc0_strong_mono with "Hwpc"); auto.
   iSplit; last first.
   { iIntros "$ !>". iSplitL "HP1".
-    - iSplitR; first eauto. iApply wpc_crash_modality_intro. iApply "Hwand1". eauto.
-    - iApply "Hwand2". eauto.
+    - iSplitR; first eauto. iApply wpc_crash_modality_intro. iApply "Hw3". iApply "Hw1". iApply "Hw2". eauto.
+    - iApply "Hw3'". iApply "Hw1'". iApply "Hw2'". eauto.
   }
   iIntros (v) "Hc' !> Htok".
 
   iDestruct ("Htok") as "(Htok1&Htok)".
   iDestruct ("Htok") as "(Htok2&Htok)".
-  iMod ("HwandP" with "[$]") as "HP".
+  iMod ("HwandP" with "[HP1 HP2]") as "HP".
+  { iSplitL "HP1".
+    - iApply "Hw2". eauto.
+    - iApply "Hw2'". eauto. }
   assert (∃ mj0, /2 < mj0 ∧ mj0 < mj_wp1 `min` mj_wp2)%Qp as (mj0&Hmj0).
   {
     apply Qp_lt_densely_ordered.
@@ -467,7 +508,8 @@ Proof.
   iMod "Hclo" as "_". iModIntro.
 
   iSplitL "Hcancel2".
-  { iApply (wpc_crash_modality_strong_wand with "Hcancel2"); auto.
+  { iApply (wpc_crash_modality_strong_wand with "Hcancel2"); auto; last first.
+    { iIntros. iModIntro. iApply "Hw3'". iFrame. }
     split.
     - apply Qp_min_glb1_lt; auto.
     - apply Qp_le_min_r.
@@ -476,7 +518,7 @@ Proof.
   iDestruct ("Htok") as "(Htok1&Htok)".
   iDestruct ("Htok") as "(Htok2&Htok)".
   iSpecialize ("Hc'" with "[Hval Htok1 Htok2]").
-  { iFrame "Hval Htok1". eauto. }
+  { iExists _, _. iFrame "Hval Htok1 #". iSplit; eauto. }
 
   iSplit.
   { iApply wpc_crash_modality_intro.
@@ -487,6 +529,7 @@ Proof.
       - apply Qp_min_glb1_lt; auto.
       - apply Qp_le_min_l.
     }
+    { iIntros. iModIntro. iApply "Hw3". iFrame. }
   }
 
   iSplitL "Hcancel1".
@@ -495,11 +538,40 @@ Proof.
       - apply Qp_min_glb1_lt; auto.
       - apply Qp_le_min_l.
     }
+    { iIntros. iModIntro. iApply "Hw3". iFrame. }
   }
 
  iSplit.
  - iDestruct "Hc'" as "(Hc'&_)". iApply wpc_crash_modality_intro. auto.
  - iDestruct "Hc'" as "(_&$)". eauto.
+Qed.
+
+Lemma wpc_crash_borrow_open_modify k E1 e Φ Φc P Pc:
+  to_val e = None →
+  crash_borrow P Pc -∗
+  (Φc ∧ (P -∗ WPC e @ k; E1
+                    {{λ v, ∃ P', P' ∗ □ (P' -∗ Pc) ∗ (crash_borrow P' Pc -∗ (Φc ∧ Φ v))}}
+                    {{ Φc ∗ Pc }})) -∗
+  WPC e @ k; E1 {{ Φ }} {{ Φc }}.
+Proof.
+  iIntros (Hnv) "H1 Hwp".
+  iDestruct "H1" as (??) "(#Hw1&#Hw2&#Hw3&Hval&Hltok)".
+  iApply (wpc_staged_inv with "[$Hval Hwp Hltok]").
+  { auto. }
+  iSplit.
+  { iDestruct "Hwp" as "($&_)". }
+  iIntros "HP".
+  iDestruct "Hwp" as "(_&Hwp)".
+  iSpecialize ("Hwp" with "[HP]").
+  { iApply "Hw2". eauto. }
+  iApply (wpc_strong_mono with "Hwp"); auto.
+  { iSplit; last first.
+    { iIntros "($&?) !>". iApply "Hw3". eauto. }
+    iIntros (?). iDestruct 1 as (P') "(HP&#Hwand&H)". iModIntro.
+    iExists P'. iFrame. iSplit.
+    { iModIntro. iIntros. iApply "Hw3". iApply "Hwand". eauto. }
+    iIntros "Hs".
+    iApply "H". iExists _, _. iFrame "Hs # ∗". eauto. }
 Qed.
 
 Lemma wpc_crash_borrow_open k E1 e Φ Φc P Pc:
@@ -511,21 +583,23 @@ Lemma wpc_crash_borrow_open k E1 e Φ Φc P Pc:
   WPC e @ k; E1 {{ Φ }} {{ Φc }}.
 Proof.
   iIntros (Hnv) "H1 Hwp".
-  iDestruct "H1" as "(#Hwand&Hval&Hltok)".
+  iDestruct "H1" as (??) "(#Hw1&#Hw2&#Hw3&Hval&Hltok)".
   iApply (wpc_staged_inv with "[$Hval Hwp Hltok]").
   { auto. }
   iSplit.
   { iDestruct "Hwp" as "($&_)". }
   iIntros "HP".
   iDestruct "Hwp" as "(_&Hwp)".
-  iSpecialize ("Hwp" with "[$]").
+  iSpecialize ("Hwp" with "[HP]").
+  { iApply "Hw2". eauto. }
   iApply (wpc_strong_mono with "Hwp"); auto.
-  { iSplit; last eauto.
+  { iSplit; last first.
+    { iIntros "($&?) !>". iApply "Hw3". eauto. }
     iIntros (?) "(HP&H)". iModIntro.
     iExists P. iFrame. iSplit.
-    { iModIntro. iIntros. by iApply "Hwand". }
+    { iModIntro. iIntros. iApply "Hw3". by iApply "Hw1". }
     iIntros "Hs".
-    iApply "H". iFrame "# ∗". }
+    iApply "H". iExists _, _. iFrame "Hs # ∗". eauto. }
 Qed.
 
 End crash_borrow_def.
